RocqOfRust/revm/revm_interpreter/instructions/simulate/control/stop.v
@@ -57,7 +57,7 @@ Proof.
   with_strategy transparent [run_stop] unfold stop, run_stop; cbn.
   s. {
     apply halt_eq.
-    apply InterpreterTypesEq.
+    exact InterpreterTypesEq.
   }
   s.
 Qed.
